refactor; expose the structure of "framework"

Structures/Types.v
@@ -1,50 +1,53 @@
 From Coq Require Import List.
 From Coq Require ssrbool.
 Import (coercions) ssrbool.
-From ABCProtocol Require Export Address.
+From ABCProtocol.Structures Require Export Address.
+From ABCProtocol.Utils Require Export ListFacts.
 
+Module Type Signable.
 
-Module Type Types (A : NetAddr).
-
-Import A.
-
-(* Some design choices: 
-1. receiving key or not?
-2. how to relate with history?
-3. sending key or not (use address as sending key --> let that node use its own key)
-
-on value: 
-1. total or partial function?
-2. make it a part of network or here?
-*)
+(* ideally, this would be "bytes" ... here model the objects that can be signed *)
 
 Parameter Value : Set.
 Parameter Value_eqdec : forall (v1 v2 : Value), {v1 = v2} + {v1 <> v2}.
 
-(* FIXME: it seems that value_bft, as well as the value stored in a node's state
-    will never change. maybe we only need to store one of them
-  or, only use for initialization but do not mention it afterwards?
-*)
+End Signable.
 
-Parameter value_bft : Address -> Value.
+Module Type PKI (Export A : NetAddr) (Export V : Signable).
+
+(* would expect that in this setting, an address is more or less a public key *)
 
 Parameter PrivateKey : Set.
 Parameter Signature : Set.
 Parameter Signature_eqdec : forall (s1 s2 : Signature), {s1 = s2} + {s1 <> s2}.
 
-(* TODO should this key & signature be of the same type as above? *)
+Parameter key_map : Address -> PrivateKey.
+Parameter verify : Value -> Signature -> Address -> bool.
+Parameter sign : Value -> PrivateKey -> Signature.
+
+(* symbolic security assumption *)
+
+Axiom key_correct : forall v n s, 
+  s = (sign v (key_map n)) <-> verify v s n.
+
+Fact correct_sign_verify_ok v n :
+  verify v (sign v (key_map n)) n.
+Proof. now rewrite <- key_correct. Qed.
+
+End PKI.
+
+Module Type ThresholdSignatureScheme (Export A : NetAddr) (Export V : Signable).
+
 Parameter LightPrivateKey : Set.
 Parameter LightSignature : Set.
 Parameter LightSignature_eqdec : forall (ls1 ls2 : LightSignature), {ls1 = ls2} + {ls1 <> ls2}.
 Parameter CombinedSignature : Set.
 Parameter CombinedSignature_eqdec : forall (cs1 cs2 : CombinedSignature), {cs1 = cs2} + {cs1 <> cs2}.
 
-Parameter key_map : Address -> PrivateKey.
-Parameter verify : Value -> Signature -> Address -> bool.
-Parameter sign : Value -> PrivateKey -> Signature.
-
 Parameter lightkey_map : Address -> LightPrivateKey.
-(* TODO if there is only one public key for this, should the address component be used or not? *)
+(* TODO if for threshold signature scheme there will be a separate public key, 
+    then we can only view Address as "the abstraction of publicly available information about a node"
+    rather than "a public key (in PKI infrastructure)" *)
 Parameter light_verify : Value -> LightSignature -> Address -> bool.
 Parameter light_sign : Value -> LightPrivateKey -> LightSignature.
 (* use dependent type to restrict the number of light signatures *)
@@ -52,11 +55,21 @@ Parameter light_sign : Value -> LightPrivateKey -> LightSignature.
 (* TODO using dependent type may incur difficulty in the protocol, so use a total function at first 
   if the number of light certificates is not (N-t0), then simply return some garbage
   (guaranteed by "combine_correct" below) *)
+(*
+(* it might also be good to know who signed these shared signatures, 
+    without which we may be unable to implement the TSS
+    by using the original PKI infrastructure; 
+  also, theoretically we should be allowed to know the signers? *)
+Parameter lightsig_combine : list (Address * LightSignature) -> CombinedSignature.
+
+(* or, we can bake the information of sender into LightSignature *)
+(* or, we can make the information of sender optional *)
+(* FIXME: read some real-world code of TSS to make decision *)
+*)
 Parameter lightsig_combine : list LightSignature -> CombinedSignature.
 Parameter combined_verify : Value -> CombinedSignature -> bool.
 
-Axiom key_correct : forall v n s, 
-  s = (sign v (key_map n)) <-> verify v s n.
+(* symbolic security assumption *)
 
 Axiom lightkey_correct : forall v n ls, 
   ls = (light_sign v (lightkey_map n)) <-> light_verify v ls n.
@@ -67,223 +80,108 @@ Axiom combine_correct : forall v cs,
     cs = lightsig_combine (map (fun n => light_sign v (lightkey_map n)) ns)) 
   <-> combined_verify v cs.
 
-Fact correct_sign_verify_ok v n :
-  verify v (sign v (key_map n)) n.
-Proof. now rewrite <- key_correct. Qed.
-
 Fact correct_sign_verify_ok_light v n :
   light_verify v (light_sign v (lightkey_map n)) n.
 Proof. now rewrite <- lightkey_correct. Qed.
 
-(* temporarily use list; there should be some notation of finite multisets or ...? *)
+End ThresholdSignatureScheme. 
 
-Definition AddrSigPair_eqdec : forall (nsig1 nsig2 : Address * Signature), {nsig1 = nsig2} + {nsig1 <> nsig2}.
-  intros. decide equality.
-  - apply Signature_eqdec. 
-  - apply Address_eqdec.
-Qed. 
+(*
+Module SimpleTSS (A : NetAddr) (V : Signable) (P : PKI A V).
 
-Definition AddrLightSigPair_eqdec : forall (nsig1 nsig2 : Address * LightSignature), {nsig1 = nsig2} + {nsig1 <> nsig2}.
-  intros. decide equality.
-  - apply LightSignature_eqdec. 
-  - apply Address_eqdec.
-Qed. 
+(* use PKI to emulate TSS *)
 
-Definition Certificate : Type := Value * list (Address * Signature).
-Definition LightCertificate : Type := Value * CombinedSignature.
+Import A V P.
 
-Definition Certificate_eqdec : forall (c1 c2 : Certificate), {c1 = c2} + {c1 <> c2}.
-  intros. decide equality. 1: do 2 (decide equality).
-  - apply Signature_eqdec. 
-  - apply Address_eqdec.
-  - apply Value_eqdec.
-Qed. 
+(* in this case, need to include the information of senders somewhere, 
+    otherwise cannot use the original verify function *)
 
-Definition LightCertificate_eqdec : forall (c1 c2 : LightCertificate), {c1 = c2} + {c1 <> c2}.
-  intros. decide equality.
-  - apply CombinedSignature_eqdec. 
-  - apply Value_eqdec.
-Qed. 
+Definition LightPrivateKey := PrivateKey.
+Definition LightSignature := (Address * Signature)%type.
+Definition LightSignature_eqdec := prod_eq_dec Address_eqdec Signature_eqdec.
 
-Parameter lightcert_conflict_check : list LightCertificate -> bool.
-Parameter genproof : list Certificate -> list Address.
+Definition CombinedSignature := list LightSignature. 
+Definition CombinedSignature_eqdec : forall (cs1 cs2 : CombinedSignature), {cs1 = cs2} + {cs1 <> cs2}.
+  intros.
+  apply list_eq_dec, LightSignature_eqdec.
+Defined.
 
-Definition lightcert_conflict_check_spec (lcc : list LightCertificate -> bool) : Prop :=
-  forall lcerts, lcc lcerts <-> 
-    exists v1 v2 cs1 cs2,
-      v1 <> v2 /\
-      In (v1, cs1) lcerts /\
-      In (v2, cs2) lcerts.
+Definition lightkey_map := key_map.
+Definition light_verify v lsig n := 
+  if Address_eqdec n (fst lsig) then verify v (snd lsig) n else false.
+Definition light_sign v pk := (* ! *).
+(*
+(* TODO where to add the guard checking? *)
+Definition lightsig_combine : list (Address * LightSignature) -> CombinedSignature := id.
+Definition combined_verify (v : Value) (cs : CombinedSignature) :=
+  forallb (fun '(n, lsig) => light_verify v lsig n) cs.
 
-Axiom lightcert_conflict_check_correct : lightcert_conflict_check_spec lightcert_conflict_check.
+Lemma lightkey_correct : forall v n ls, 
+  ls = (light_sign v (lightkey_map n)) <-> light_verify v ls n.
+Proof key_correct.
 
-Definition genproof_can_detect (genproof : list Certificate -> list Address) : Prop :=
-  forall certs n, In n (genproof certs) <-> 
-    exists v1 v2 sig1 sig2 nsigs1 nsigs2,
-      v1 <> v2 /\
-      In (v1, nsigs1) certs /\
-      In (v2, nsigs2) certs /\
-      In (n, sig1) nsigs1 /\
-      In (n, sig2) nsigs2.
-
-Record genproof_spec (genproof : list Certificate -> list Address) : Prop := {
-  _ : genproof_can_detect genproof;
-  _ : forall certs, NoDup (genproof certs)
-}.
-
-Axiom genproof_correct : genproof_spec genproof.
-
-(* should give concrete checkers which does not depend on knowing
-    key_map so that it is not vacuous
-  TODO for now simply keep them here
+Lemma combine_correct : forall v cs, 
+  (exists ns : list Address, 
+    NoDup ns /\ length ns = N - t0 /\
+    cs = lightsig_combine (map (fun n => (n, light_sign v (lightkey_map n))) ns)) 
+  <-> combined_verify v cs.
+Proof.
 *)
 
-Fixpoint lcc_simple_aux (v : Value) (certs : list LightCertificate) : bool :=
-  match certs with 
-  | nil => false 
-  | (v', _) :: certs' => if Value_eqdec v v' then lcc_simple_aux v certs' else true 
-  end.
+End SimpleTSS. 
+*)
 
-Fixpoint lcc_simple (certs : list LightCertificate) : bool :=
-  match certs with
-  | nil => false
-  | (v, _) :: certs' => (lcc_simple_aux v certs') || (lcc_simple certs')
-  end.
+Module Type MessageType.
 
-Lemma lcc_simple_aux_can_detect v certs : 
-  lcc_simple_aux v certs <-> exists v' cs', v <> v' /\ In (v', cs') certs.
-Proof with (first [ intuition congruence; fail | firstorder; fail | idtac ]).
-  induction certs as [ | (v', cs') certs IH ]; simpl.
-  - split...
-  - destruct (Value_eqdec v v') as [ <- | Hvneq ]...
-    + rewrite IH.
-      firstorder.
-      congruence...
-    + split...
-      intros _.
-      eauto.
+Parameter Message : Type.
+Parameter Message_eqdec : forall (m1 m2 : Message), {m1 = m2} + {m1 <> m2}.
+
+End MessageType.
+
+Module Type PacketType.
+
+Parameter Packet : Type.
+Parameter Packet_eqdec : forall (p1 p2 : Packet), {p1 = p2} + {p1 <> p2}.
+
+End PacketType.
+
+Module Type SimplePacket (Export A : NetAddr) (Export M : MessageType) <: PacketType.
+
+Record Packet_ : Type := mkP { src: Address; dst: Address; msg: Message; consumed: bool }.
+
+Definition Packet := Packet_. (* TODO this is bad! required by the module type *)
+(* Global Arguments Packet : simpl never. *)
+
+Definition Packet_eqdec : forall (p1 p2 : Packet), {p1 = p2} + {p1 <> p2}.
+  intros. 
+  decide equality; auto using Bool.bool_dec, Message_eqdec, Address_eqdec.
 Qed.
 
-Lemma lcc_simple_correct : lightcert_conflict_check_spec lcc_simple.
-Proof with (first [ intuition congruence; fail | firstorder; fail | idtac ]).
-  hnf.
-  intros.
-  induction lcerts as [ | (v, cs) lcerts IH ]; simpl.
-  - split...
-  - destruct (lcc_simple_aux v lcerts) eqn:E.
-    + split...
-      intros _.
-      apply lcc_simple_aux_can_detect in E.
-      destruct E as (v' & cs' & Hvneq & Hin).
-      exists v, v', cs, cs'...
-    + simpl.
-      pose proof (lcc_simple_aux_can_detect v lcerts) as HH.
-      unfold is_true in HH.
-      rewrite <- Bool.not_true_iff_false, -> HH in E.
-      rewrite IH.
-      split.
-      * intros (v1 & v2 & cs1 & cs2 & Hvneq & Hin1 & Hin2).
-        exists v1, v2, cs1, cs2...
-      * intros (v1 & v2 & cs1 & cs2 & Hvneq & [ E1 | Hin1 ] & [ E2 | Hin2 ]).
-        1: idtac...
-        1-2: try inversion E1; try inversion E2; subst.
-        1-2: exfalso; apply E; eauto.
-        exists v1, v2, cs1, cs2...
-Qed.
+Definition receive_pkt p :=
+  let: mkP src dst msg _ := p in mkP src dst msg true.
 
-Definition genproof_simple_aux_aux (c : Certificate) (certs : list Certificate) :=
-  (List.flat_map 
-    (fun c' => if Value_eqdec (fst c) (fst c') 
-                then nil 
-                else (filter 
-                  (fun n => In_dec Address_eqdec n (map fst (snd c))) 
-                  (map fst (snd c')))) certs).
+Definition pkt_le p p' : Prop := p' = p \/ p' = receive_pkt p (* may be redundant, but make things simpler? *).
 
-Fixpoint genproof_simple_aux (certs : list Certificate) : list Address :=
-  match certs with
-  | nil => nil
-  | c :: certs' => (genproof_simple_aux_aux c certs') ++ (genproof_simple_aux certs')
-  end.
+Fact receive_pkt_intact p (H : consumed p) : receive_pkt p = p.
+Proof. destruct p; simpl in *; now rewrite H. Qed.
 
-Definition genproof_simple (certs : list Certificate) : list Address :=
-  nodup Address_eqdec (genproof_simple_aux certs).
+Fact receive_pkt_intact_inv p (H : receive_pkt p = p) : consumed p.
+Proof. destruct p; simpl in *; congruence. Qed.
 
-Lemma genproof_simple_aux_aux_can_detect v nsigs certs n : 
-  In n (genproof_simple_aux_aux (v, nsigs) certs) <-> 
-  exists v' nsigs',
-    v <> v' /\
-    In (v', nsigs') certs /\
-    In n (map fst nsigs) /\
-    In n (map fst nsigs').
-Proof.
-  induction certs as [ | (v_, nsigs_) certs IH ].
-  - firstorder.
-  - simpl.
-    rewrite -> in_app_iff, -> IH.
-    clear IH.
-    destruct (Value_eqdec v v_) as [ <- | Hvneq ].
-    + firstorder.
-      congruence.
-    + rewrite -> filter_In.
-      (* awkward ... *)
-      assert (in_dec Address_eqdec n (map fst nsigs) <-> In n (map fst nsigs)) as Hp.
-      {
-        unfold is_true.
-        now destruct (in_dec Address_eqdec n (map fst nsigs)).
-      }
-      rewrite -> Hp.
-      intuition firstorder congruence.
-Qed.
+Fact receive_pkt_idem p : receive_pkt (receive_pkt p) = receive_pkt p.
+Proof. now destruct p. Qed.
 
-Lemma genproof_simple_aux_can_detect certs n : In n (genproof_simple_aux certs) <-> 
-  exists v1 v2 nsigs1 nsigs2,
-    v1 <> v2 /\
-    In (v1, nsigs1) certs /\
-    In (v2, nsigs2) certs /\
-    In n (map fst nsigs1) /\
-    In n (map fst nsigs2).
-Proof.
-  induction certs as [ | (v, nsigs) certs IH ].
-  - firstorder.
-  - simpl.
-    rewrite -> in_app_iff, -> IH, -> genproof_simple_aux_aux_can_detect.
-    clear IH.
-    split.
-    + intros [ (v' & nsigs' & Hvneq & Hin' & Hin_nsigs & Hin_nsigs') | 
-        (v1 & v2 & nsigs1 & nsigs2 & Hvneq & Hin1 & Hin2 & Hin_nsigs1 & Hin_nsigs2) ].
-      * exists v, v', nsigs, nsigs'.
-        intuition.
-      * exists v1, v2, nsigs1, nsigs2.
-        intuition.
-    + intros (v1 & v2 & nsigs1 & nsigs2 & Hvneq & [ Hin1 | Hin1 ] & [ Hin2 | Hin2 ] & Hin_nsigs1 & Hin_nsigs2).
-      all: try congruence.
-      1-2: left.
-      1: exists v2, nsigs2.
-      2: exists v1, nsigs1.
-      1-2: intuition congruence.
-      right.
-      exists v1, v2, nsigs1, nsigs2.
-      intuition.
-Qed.
+Definition broadcast (src : Address) (m : Message) :=
+  (map (fun x => mkP src x m false) valid_nodes).
 
-Lemma genproof_simple_correct : genproof_spec genproof_simple.
-Proof.
-  unfold genproof_simple.
-  constructor.
-  - hnf.
-    intros.
-    rewrite -> nodup_In, -> genproof_simple_aux_can_detect.
-    repeat setoid_rewrite -> in_map_iff.
-    split.
-    + intros (v1 & v2 & nsigs1 & nsigs2 & ? & ? & ? & ((n', sig1) & Htmp1 & ?) & ((n'', sig2) & Htmp2 & ?)).
-      simpl in Htmp1, Htmp2.
-      subst n' n''.
-      now exists v1, v2, sig1, sig2, nsigs1, nsigs2.
-    + intros (v1 & v2 & sig1 & sig2 & nsigs1 & nsigs2 & ? & ? & ? & ? & ?).
-      exists v1, v2, nsigs1, nsigs2.
-      firstorder.
-  - intros. 
-    now apply NoDup_nodup.
-Qed.
+Fact In_broadcast src m p :
+  In p (broadcast src m) <-> exists dst, p = mkP src dst m false.
+Proof. unfold broadcast. rewrite -> in_map_iff. pose proof Address_is_finite. firstorder; eauto. Qed.
 
-End Types.
+End SimplePacket.
+
+Module SimplePacketImpl (Export A : NetAddr) (Export M : MessageType) <: (SimplePacket A M) <: PacketType.
+
+Include SimplePacket A M.
+
+End SimplePacketImpl.
