Systems/Protocol.v
@@ -2,254 +2,29 @@ From Coq Require Import Bool List.
 From Coq Require ssrbool ssreflect.
 Import (coercions) ssrbool.
 Import ssreflect.SsrSyntax.
-From ABCProtocol Require Import Types Address ListFacts.
+From ABCProtocol.Structures Require Export Types.
 
-Module Type ACProtocol (A : NetAddr) (T : Types A).
-Import T A.
+Module Type Protocol (Export A : NetAddr) (Export M : MessageType) (Export P : PacketType).
 
-Inductive Message := 
-  | SubmitMsg (v : Value) (ls : LightSignature) (s : Signature)
-  | LightConfirmMsg (c : LightCertificate)
-  (* for historical reasons, this remains the name as "ConfirmMsg". *)
-  | ConfirmMsg (c : Certificate).
+Parameter InternalTransition : Type.
 
-Definition Message_eqdec : forall (m1 m2 : Message), {m1 = m2} + {m1 <> m2}.
-  intros. decide equality.
-  - apply Signature_eqdec.
-  - apply LightSignature_eqdec.
-  - apply Value_eqdec.
-  - apply LightCertificate_eqdec.
-  - apply Certificate_eqdec.
-Qed.
+Parameter State : Type.
+Parameter State_eqdec : forall (s1 s2 : State), {s1 = s2} + {s1 <> s2}.
 
-(* did not define msg type; seemingly it is not used in Toychain *)
+Parameter Init : Address -> State.
 
-(* only submit its own value so remember its node id is sufficient *)
+(* TODO later change this name to the more canonical "procMsg" *)
+Parameter procMsgWithCheck : State -> Address (* sender *) -> Message -> State * list Packet.
+Parameter procInt : State -> InternalTransition -> State * list Packet.
 
-Inductive InternalTransition :=
-  | SubmitIntTrans.
-(* TODO 
-    If the light certificate conflict check is modelled as an internal transition, 
-    then possibly the "eventual Byzantine detection" cannot be expressed easily. 
+End Protocol.
 
-    However, in order to trigger the check, the conf must be true (which is due to the delivery
-    of the (N-t0)-th submit message) and there must be two conflicting light certificates
-    (which is due to the delivery of some LightConfirmMsg).  
+(*
+Module Type Protocol' (Export A : NetAddr) (Export M : MessageType) (Export P : SimplePacket A M)(* <: Protocol A M P *).
 
-    They are not synchronized, so we should append "monitors" to the above
-    two delivery actions, if not to make light certificate check internal. 
+(* if do not use this instantiation, then Protocol' is essentially Protocol? *)
+(* Module Export P <: PacketType := SimplePacketImpl A M. *)
+Include (Protocol A M P).
 
-    This is troublesome for now. I suppose there would be a better way to systematically 
-    frame out such monitors in the proof (maybe IVy has done something similar). 
-
-  Wait. This may be done with a new kind of transitions?
+End Protocol'.
 *)
-
-Record Packet := mkP {src: Address; dst: Address; msg: Message; consumed: bool}.
-
-Definition receive_pkt p :=
-  let: mkP src dst msg _ := p in mkP src dst msg true.
-
-Definition pkt_le p p' : Prop := p' = p \/ p' = receive_pkt p (* may duplicate, but make things simpler? *).
-
-Fact receive_pkt_intact p : consumed p = true <-> receive_pkt p = p.
-Proof. destruct p; simpl; split; congruence. Qed.
-
-Fact receive_pkt_idem p : receive_pkt (receive_pkt p) = receive_pkt p.
-Proof. now destruct p. Qed.
-
-Definition Packet_eqdec : forall (p1 p2 : Packet), {p1 = p2} + {p1 <> p2}.
-  intros. decide equality.
-  - decide equality.
-  - apply Message_eqdec.
-  - apply Address_eqdec.
-  - apply Address_eqdec.
-Qed.
-
-(* TODO assume peers are already known? *)
-
-Record State :=
-  Node {
-    id : Address;
-    (* peers : peers_t; *)
-    conf : bool;
-    submitted_value : option Value;
-    (* need to contain all addresses otherwise cannot perform operations like set *)
-    (* since there are two kinds of signatures now, seems cannot avoid using split/combine *)
-    from_set : list Address;
-    collected_lightsigs : list LightSignature;
-    collected_sigs : list Signature;
-    received_lightcerts : list LightCertificate;
-    received_certs : list Certificate;
-    (* holding all pending submit messages *)
-    (* TODO add it here, or in a separate State type? *)
-    msg_buffer : list (Address * Message)
-  }.
-
-Definition State_eqdec : forall (s1 s2 : State), {s1 = s2} + {s1 <> s2}.
-  intros. decide equality.
-  - decide equality. decide equality; [ apply Message_eqdec | apply Address_eqdec ].
-  - decide equality. apply Certificate_eqdec.
-  - decide equality. apply LightCertificate_eqdec.
-  - decide equality. apply Signature_eqdec.
-  - decide equality. apply LightSignature_eqdec.
-  - decide equality. apply Address_eqdec.
-  - decide equality. apply Value_eqdec.
-  - decide equality.
-  - apply Address_eqdec.
-Qed.
-
-Definition Init (n : Address) : State :=
-  Node n false None nil nil nil nil nil nil.
-
-Definition broadcast (src : Address) (m : Message) :=
-  (map (fun x => mkP src x m false) valid_nodes).
-
-Fact In_broadcast src m p :
-  In p (broadcast src m) <-> exists dst, p = mkP src dst m false.
-Proof. unfold broadcast. rewrite -> in_map_iff. pose proof Address_is_finite. firstorder; eauto. Qed.
-
-Definition certificate_valid v nsigs : Prop :=
-  Forall (fun '(n, sig) => verify v sig n) nsigs.
-
-Definition verify_certificate v nsigs : {certificate_valid v nsigs} + {~ certificate_valid v nsigs}.
-  unfold certificate_valid.
-  apply Forall_dec. (* there is no existing Forall2_dec *)
-  intros (n, sig).
-  apply bool_dec.
-Qed.
-
-Definition light_signatures_valid v nlsigs : Prop :=
-  Forall (fun '(n, lsig) => light_verify v lsig n) nlsigs.
-
-Fact light_signatures_valid_for_combine v ns lsigs
-  (Hlen : length ns = length lsigs) (H : light_signatures_valid v (combine ns lsigs)) :
-  lsigs = map (fun n => light_sign v (lightkey_map n)) ns.
-Proof.
-  apply length_eq_Forall2_True in Hlen.
-  induction Hlen as [ | n ls ns lsigs _ _ IH ].
-  - reflexivity.
-  - simpl in H.
-    apply Forall_cons_iff in H.
-    destruct H as (->%lightkey_correct & H).
-    specialize (IH H).
-    subst lsigs.
-    split; auto.
-Qed.
-
-Definition zip_from_lsigs (st : State) := 
-  List.combine st.(from_set) st.(collected_lightsigs).
-
-Definition zip_from_sigs (st : State) := 
-  List.combine st.(from_set) st.(collected_sigs).
-
-Definition zip_from_lsigs_sigs (st : State) := 
-  List.combine (List.combine st.(from_set) st.(collected_lightsigs)) st.(collected_sigs).
-
-(* there is only one such check, so somewhat ad-hoc *)
-(* TODO remove the let binding here? *)
-(* FIXME: possibly make sure this would be triggered only once *)
-Definition routine_check (st : State) : list Packet :=
-  let: Node n conf ov from lsigs sigs rlcerts rcerts buffer := st in
-  match ov with 
-  | Some vthis => 
-    (* actually confirmation implies submission; but we need to use vthis so anyway *)
-    if conf
-    then 
-      (if lightcert_conflict_check rlcerts
-      then broadcast n (ConfirmMsg (vthis, zip_from_sigs st))
-      else nil)
-    else nil
-  | None => nil
-  end
-.
-
-Definition procMsg (st : State) (src : Address) (msg : Message) : State * list Packet :=
-  let: Node n conf ov from lsigs sigs rlcerts rcerts buffer := st in
-  match msg with
-  | SubmitMsg v lsig sig =>
-    match ov with 
-    | Some vthis => 
-      if Value_eqdec v vthis 
-      then
-        (* just to clarify: in the paper, this check is subsumed by Line 6 *)
-        (if verify v sig src
-        then 
-          (if light_verify v lsig src
-          then 
-            (* before prepending, add a check to avoid adding a duplicate node-signature pair *)
-            (* checking In fst or In pair should be the same, due to the correctness of verify *)
-            (* prevent enlarging from_set after confirmation; TODO need to align this with paper? seems not ... *)
-            (* let: in_from := In_dec Address_eqdec src (map fst nsigs) in *)
-            let: in_from := In_dec Address_eqdec src from in
-            let: from' := if conf || in_from then from else src :: from in
-            let: lsigs' := if conf || in_from then lsigs else lsig :: lsigs in
-            let: sigs' := if conf || in_from then sigs else sig :: sigs in
-            (* let: conf' := (Nat.leb (N - t0) (length from')) in *)
-            let: conf' := conf || (Nat.leb (N - t0) (length from')) in
-            let: ps := (if conf' 
-              then broadcast n (LightConfirmMsg (v, lightsig_combine lsigs'))
-              else nil) in
-            let: st' := Node n conf' ov from' lsigs' sigs' rlcerts rcerts buffer in
-            (st', ps)
-          else (st, nil))
-        else (st, nil))
-      else (st, nil)
-    | None => 
-      (* add to the buffer and wait *)
-      (Node n conf ov from lsigs sigs rlcerts rcerts ((src, msg) :: buffer), nil)
-    end
-  | LightConfirmMsg lc =>
-    let: (v, cs) := lc in
-    if combined_verify v cs
-    then 
-      let: st' := Node n conf ov from lsigs sigs (lc :: rlcerts) rcerts buffer in
-      (st', nil)
-    else (st, nil)
-  | ConfirmMsg c => 
-    let: (v, nsigs) := c in
-    (* check whether this is a valid full certificate or not *)
-    (* in the paper this condition is ">= N-t0 distinct senders", 
-        which is stronger than this *)
-    if NoDup_eqdec AddrSigPair_eqdec nsigs
-    then 
-      (if Nat.leb (N - t0) (length nsigs) 
-      then
-        (if verify_certificate v nsigs
-        then 
-          let: st' := Node n conf ov from lsigs sigs rlcerts (c :: rcerts) buffer in
-          (st', nil)
-        else (st, nil))
-      else (st, nil))
-    else (st, nil)
-  end.
-
-(* a simple wrapper *)
-
-Definition procMsgWithCheck (st : State) (src : Address) (msg : Message) : State * list Packet :=
-  let: (st', ps) := procMsg st src msg in
-  (* a minor optimization? *)
-  match msg with
-  | SubmitMsg _ _ _ | LightConfirmMsg _ => (st', routine_check st' ++ ps)
-  | _ => (st', ps)
-  end.
-
-Definition procInt (st : State) (tr : InternalTransition) :=
-  let: Node n conf ov from lsigs sigs rlcerts rcerts buffer := st in
-  match tr with
-  | SubmitIntTrans => 
-    (* TODO constrain this to happen at most once? *)
-    let: vthis := value_bft n in
-    let: ps := broadcast n 
-      (SubmitMsg vthis (light_sign vthis (lightkey_map n)) (sign vthis (key_map n))) in
-    (* also start to process all messages in the buffer *)
-    (* not putting ps into the initial value of fold should be easier? *)
-    let: (st', ps') := 
-      fold_right
-        (fun nmsg stps => let: (res1, res2) := procMsgWithCheck (fst stps) (fst nmsg) (snd nmsg) in
-          (res1, res2 ++ snd stps)) 
-        (Node n conf (Some vthis) from lsigs sigs rlcerts rcerts nil, nil) buffer in
-    (st', ps' ++ ps)  
-  end.
-
-End ACProtocol.
