Protocols/ABC/Protocol.v
@@ -1,0 +1,227 @@
+From Coq Require Import Bool List.
+From Coq Require ssrbool.
+Import (coercions) ssrbool.
+From ABCProtocol.Systems Require Export Protocol.
+From ABCProtocol.Protocols.ABC Require Export Types.
+
+Module Type ACProtocol (A : NetAddr) (V : Signable) (VBFT : ValueBFT A V) 
+  (P : PKI A V) (TSS : ThresholdSignatureScheme A V)
+  (ACDT : ACDataTypes A V P TSS) 
+  (CC : CertCheckers A V P TSS ACDT) (M : ACMessage A V P TSS ACDT)
+  (P0 : SimplePacket A M) <: Protocol A M P0.
+
+Import A V VBFT P TSS ACDT CC M P0.
+
+Inductive InternalTransition_ :=
+  | SubmitIntTrans.
+
+Definition InternalTransition := InternalTransition_.
+(* TODO 
+    If the light certificate conflict check is modelled as an internal transition, 
+    then possibly the "eventual Byzantine detection" cannot be expressed easily. 
+
+    However, in order to trigger the check, the conf must be true (which is due to the delivery
+    of the (N-t0)-th submit message) and there must be two conflicting light certificates
+    (which is due to the delivery of some LightConfirmMsg).  
+
+    They are not synchronized, so we should append "monitors" to the above
+    two delivery actions, if not to make light certificate check internal. 
+
+    This is troublesome for now. I suppose there would be a better way to systematically 
+    frame out such monitors in the proof (maybe IVy has done something similar). 
+
+  Wait. This may be done with a new kind of transitions?
+*)
+
+(* TODO assume peers are already known? *)
+
+Record State_ :=
+  Node {
+    id : Address;
+    (* peers : peers_t; *)
+    conf : bool;
+    submitted_value : option Value;
+    (* need to contain all addresses otherwise cannot perform operations like set *)
+    (* since there are two kinds of signatures now, seems cannot avoid using split/combine *)
+    from_set : list Address;
+    collected_lightsigs : list LightSignature;
+    collected_sigs : list Signature;
+    received_lightcerts : list LightCertificate;
+    received_certs : list Certificate;
+    (* holding all pending submit messages *)
+    (* TODO add it here, or in a separate State type? *)
+    msg_buffer : list (Address * Message)
+  }.
+
+Definition State := State_.
+
+Definition State_eqdec : forall (s1 s2 : State), {s1 = s2} + {s1 <> s2}.
+  intros. decide equality.
+  - decide equality. apply prod_eq_dec; auto using Message_eqdec, Address_eqdec.
+  - decide equality. apply Certificate_eqdec.
+  - decide equality. apply LightCertificate_eqdec.
+  - decide equality. apply Signature_eqdec.
+  - decide equality. apply LightSignature_eqdec.
+  - decide equality. apply Address_eqdec.
+  - decide equality. apply Value_eqdec.
+  - decide equality.
+  - apply Address_eqdec.
+Qed.
+
+Definition Init (n : Address) : State :=
+  Node n false None nil nil nil nil nil nil.
+
+Definition certificate_valid v nsigs : Prop :=
+  Forall (fun '(n, sig) => verify v sig n) nsigs.
+
+Definition verify_certificate v nsigs : {certificate_valid v nsigs} + {~ certificate_valid v nsigs}.
+  unfold certificate_valid.
+  apply Forall_dec. (* there is no existing Forall2_dec *)
+  intros (n, sig).
+  apply bool_dec.
+Qed.
+
+Definition light_signatures_valid v nlsigs : Prop :=
+  Forall (fun '(n, lsig) => light_verify v lsig n) nlsigs.
+
+Fact light_signatures_valid_for_combine v ns lsigs
+  (Hlen : length ns = length lsigs) (H : light_signatures_valid v (combine ns lsigs)) :
+  lsigs = map (fun n => light_sign v (lightkey_map n)) ns.
+Proof.
+  apply length_eq_Forall2_True in Hlen.
+  induction Hlen as [ | n ls ns lsigs _ _ IH ].
+  - reflexivity.
+  - simpl in H.
+    apply Forall_cons_iff in H.
+    destruct H as (->%lightkey_correct & H).
+    specialize (IH H).
+    subst lsigs.
+    split; auto.
+Qed.
+
+Definition zip_from_lsigs (st : State) := 
+  List.combine st.(from_set) st.(collected_lightsigs).
+
+Definition zip_from_sigs (st : State) := 
+  List.combine st.(from_set) st.(collected_sigs).
+
+Definition zip_from_lsigs_sigs (st : State) := 
+  List.combine (List.combine st.(from_set) st.(collected_lightsigs)) st.(collected_sigs).
+
+(* there is only one such check, so somewhat ad-hoc *)
+(* TODO remove the let binding here? *)
+(* FIXME: possibly make sure this would be triggered only once *)
+Definition routine_check (st : State) : list Packet :=
+  let: Node n conf ov from lsigs sigs rlcerts rcerts buffer := st in
+  match ov with 
+  | Some vthis => 
+    (* actually confirmation implies submission; but we need to use vthis so anyway *)
+    if conf
+    then 
+      (if lightcert_conflict_check rlcerts
+      then broadcast n (ConfirmMsg (vthis, zip_from_sigs st))
+      else nil)
+    else nil
+  | None => nil
+  end
+.
+
+Definition procMsg (st : State) (src : Address) (msg : Message) : State * list Packet :=
+  let: Node n conf ov from lsigs sigs rlcerts rcerts buffer := st in
+  match msg with
+  | SubmitMsg v lsig sig =>
+    match ov with 
+    | Some vthis => 
+      if Value_eqdec v vthis 
+      then
+        (* just to clarify: in the paper, this check is subsumed by Line 6 *)
+        (if verify v sig src
+        then 
+          (if light_verify v lsig src
+          then 
+            (* before prepending, add a check to avoid adding a duplicate node-signature pair *)
+            (* checking In fst or In pair should be the same, due to the correctness of verify *)
+            (* prevent enlarging from_set after confirmation; TODO need to align this with paper? seems not ... *)
+            (* let: in_from := In_dec Address_eqdec src (map fst nsigs) in *)
+            let: in_from := In_dec Address_eqdec src from in
+            let: from' := if conf || in_from then from else src :: from in
+            let: lsigs' := if conf || in_from then lsigs else lsig :: lsigs in
+            let: sigs' := if conf || in_from then sigs else sig :: sigs in
+            (* let: conf' := (Nat.leb (N - t0) (length from')) in *)
+            let: conf' := conf || (Nat.leb (N - t0) (length from')) in
+            let: ps := (if conf' 
+              then broadcast n (LightConfirmMsg (v, lightsig_combine lsigs'))
+              else nil) in
+            let: st' := Node n conf' ov from' lsigs' sigs' rlcerts rcerts buffer in
+            (st', ps)
+          else (st, nil))
+        else (st, nil))
+      else (st, nil)
+    | None => 
+      (* add to the buffer and wait *)
+      (Node n conf ov from lsigs sigs rlcerts rcerts ((src, msg) :: buffer), nil)
+    end
+  | LightConfirmMsg lc =>
+    let: (v, cs) := lc in
+    if combined_verify v cs
+    then 
+      let: st' := Node n conf ov from lsigs sigs (lc :: rlcerts) rcerts buffer in
+      (st', nil)
+    else (st, nil)
+  | ConfirmMsg c => 
+    let: (v, nsigs) := c in
+    (* check whether this is a valid full certificate or not *)
+    (* in the paper this condition is ">= N-t0 distinct senders", 
+        which is stronger than this *)
+    if NoDup_eqdec AddrSigPair_eqdec nsigs
+    then 
+      (if Nat.leb (N - t0) (length nsigs) 
+      then
+        (if verify_certificate v nsigs
+        then 
+          let: st' := Node n conf ov from lsigs sigs rlcerts (c :: rcerts) buffer in
+          (st', nil)
+        else (st, nil))
+      else (st, nil))
+    else (st, nil)
+  end.
+
+(* a simple wrapper *)
+
+Definition procMsgWithCheck (st : State) (src : Address) (msg : Message) : State * list Packet :=
+  let: (st', ps) := procMsg st src msg in
+  (* a minor optimization? *)
+  match msg with
+  | SubmitMsg _ _ _ | LightConfirmMsg _ => (st', routine_check st' ++ ps)
+  | _ => (st', ps)
+  end.
+
+Definition procInt (st : State) (tr : InternalTransition) :=
+  let: Node n conf ov from lsigs sigs rlcerts rcerts buffer := st in
+  match tr with
+  | SubmitIntTrans => 
+    (* TODO constrain this to happen at most once? *)
+    let: vthis := value_bft n in
+    let: ps := broadcast n 
+      (SubmitMsg vthis (light_sign vthis (lightkey_map n)) (sign vthis (key_map n))) in
+    (* also start to process all messages in the buffer *)
+    (* not putting ps into the initial value of fold should be easier? *)
+    let: (st', ps') := 
+      fold_right
+        (fun nmsg stps => let: (res1, res2) := procMsgWithCheck (fst stps) (fst nmsg) (snd nmsg) in
+          (res1, res2 ++ snd stps)) 
+        (Node n conf (Some vthis) from lsigs sigs rlcerts rcerts nil, nil) buffer in
+    (st', ps' ++ ps)  
+  end.
+
+End ACProtocol.
+
+Module ACProtocolImpl (A : NetAddr) (V : Signable) (VBFT : ValueBFT A V) 
+  (P : PKI A V) (TSS : ThresholdSignatureScheme A V)
+  (ACDT : ACDataTypes A V P TSS) 
+  (CC : CertCheckers A V P TSS ACDT) (M : ACMessage A V P TSS ACDT)
+  (P0 : SimplePacket A M) <: Protocol A M P0 <: ACProtocol A V VBFT P TSS ACDT CC M P0.
+
+Include ACProtocol A V VBFT P TSS ACDT CC M P0.
+
+End ACProtocolImpl.
