Protocols/ABC/Types.v
@@ -1,0 +1,279 @@
+From Coq Require Import List.
+From Coq Require ssrbool.
+Import (coercions) ssrbool.
+From ABCProtocol.Structures Require Export Types.
+
+Module Type ValueBFT (Export A : NetAddr) (Export V : Signable).
+
+Parameter value_bft : Address -> Value.
+
+End ValueBFT.
+
+Module Type ACDataTypes (A : NetAddr) (V : Signable) (P : PKI A V) (TSS : ThresholdSignatureScheme A V).
+
+Import A V P TSS.
+
+Definition AddrSigPair_eqdec : forall (nsig1 nsig2 : Address * Signature), {nsig1 = nsig2} + {nsig1 <> nsig2}.
+  intros. decide equality.
+  - apply Signature_eqdec. 
+  - apply Address_eqdec.
+Qed. 
+
+Definition AddrLightSigPair_eqdec : forall (nsig1 nsig2 : Address * LightSignature), {nsig1 = nsig2} + {nsig1 <> nsig2}.
+  intros. decide equality.
+  - apply LightSignature_eqdec. 
+  - apply Address_eqdec.
+Qed. 
+
+(* temporarily use list; there should be some notation of finite multisets or ...? *)
+
+Definition Certificate : Type := Value * list (Address * Signature).
+Definition LightCertificate : Type := Value * CombinedSignature.
+
+Definition Certificate_eqdec : forall (c1 c2 : Certificate), {c1 = c2} + {c1 <> c2}.
+  intros. decide equality. 1: do 2 (decide equality).
+  - apply Signature_eqdec. 
+  - apply Address_eqdec.
+  - apply Value_eqdec.
+Qed. 
+
+Definition LightCertificate_eqdec : forall (c1 c2 : LightCertificate), {c1 = c2} + {c1 <> c2}.
+  intros. decide equality.
+  - apply CombinedSignature_eqdec. 
+  - apply Value_eqdec.
+Qed. 
+
+End ACDataTypes.
+
+Module ACDataTypesImpl (A : NetAddr) (V : Signable) (P : PKI A V) (TSS : ThresholdSignatureScheme A V)
+  <: ACDataTypes A V P TSS.
+
+Include ACDataTypes A V P TSS.
+
+End ACDataTypesImpl.
+
+Module Type CertCheckers (A : NetAddr) (V : Signable) (P : PKI A V) (TSS : ThresholdSignatureScheme A V)
+  (ACDT : ACDataTypes A V P TSS).
+
+Import A V P TSS ACDT.
+
+Parameter lightcert_conflict_check : list LightCertificate -> bool.
+Parameter genproof : list Certificate -> list Address.
+
+Axiom lightcert_conflict_check_correct : 
+  forall lcerts, lightcert_conflict_check lcerts <-> 
+    exists v1 v2 cs1 cs2,
+      v1 <> v2 /\
+      In (v1, cs1) lcerts /\
+      In (v2, cs2) lcerts.
+
+Axiom genproof_correct : 
+  (forall certs, NoDup (genproof certs)) /\
+  (forall certs n, In n (genproof certs) <-> 
+    exists v1 v2 sig1 sig2 nsigs1 nsigs2,
+      v1 <> v2 /\
+      In (v1, nsigs1) certs /\
+      In (v2, nsigs2) certs /\
+      In (n, sig1) nsigs1 /\
+      In (n, sig2) nsigs2).
+
+End CertCheckers.
+
+Module CertCheckersImpl (A : NetAddr) (V : Signable) (P : PKI A V) (TSS : ThresholdSignatureScheme A V)
+  (ACDT : ACDataTypes A V P TSS) <: CertCheckers A V P TSS ACDT.
+
+Import A V P TSS ACDT.
+
+Fixpoint lcc_simple_aux (v : Value) (certs : list LightCertificate) : bool :=
+  match certs with 
+  | nil => false 
+  | (v', _) :: certs' => if Value_eqdec v v' then lcc_simple_aux v certs' else true 
+  end.
+
+Fixpoint lcc_simple (certs : list LightCertificate) : bool :=
+  match certs with
+  | nil => false
+  | (v, _) :: certs' => (lcc_simple_aux v certs') || (lcc_simple certs')
+  end.
+
+Definition lightcert_conflict_check := lcc_simple.
+
+Lemma lcc_simple_aux_can_detect v certs : 
+  lcc_simple_aux v certs <-> exists v' cs', v <> v' /\ In (v', cs') certs.
+Proof with (first [ intuition congruence; fail | firstorder; fail | idtac ]).
+  induction certs as [ | (v', cs') certs IH ]; simpl.
+  - split...
+  - destruct (Value_eqdec v v') as [ <- | Hvneq ]...
+    + rewrite IH.
+      firstorder.
+      congruence...
+    + split...
+      intros _.
+      eauto.
+Qed.
+
+Lemma lightcert_conflict_check_correct : 
+  forall lcerts, lightcert_conflict_check lcerts <-> 
+    exists v1 v2 cs1 cs2,
+      v1 <> v2 /\
+      In (v1, cs1) lcerts /\
+      In (v2, cs2) lcerts.
+Proof with (first [ intuition congruence; fail | firstorder; fail | idtac ]).
+  unfold lightcert_conflict_check.
+  intros.
+  induction lcerts as [ | (v, cs) lcerts IH ]; simpl.
+  - split...
+  - destruct (lcc_simple_aux v lcerts) eqn:E.
+    + split...
+      intros _.
+      apply lcc_simple_aux_can_detect in E.
+      destruct E as (v' & cs' & Hvneq & Hin).
+      exists v, v', cs, cs'...
+    + simpl.
+      pose proof (lcc_simple_aux_can_detect v lcerts) as HH.
+      unfold is_true in HH.
+      rewrite <- Bool.not_true_iff_false, -> HH in E.
+      rewrite IH.
+      split.
+      * intros (v1 & v2 & cs1 & cs2 & Hvneq & Hin1 & Hin2).
+        exists v1, v2, cs1, cs2...
+      * intros (v1 & v2 & cs1 & cs2 & Hvneq & [ E1 | Hin1 ] & [ E2 | Hin2 ]).
+        1: idtac...
+        1-2: try inversion E1; try inversion E2; subst.
+        1-2: exfalso; apply E; eauto.
+        exists v1, v2, cs1, cs2...
+Qed.
+
+Definition genproof_simple_aux_aux (c : Certificate) (certs : list Certificate) :=
+  (List.flat_map 
+    (fun c' => if Value_eqdec (fst c) (fst c') 
+                then nil 
+                else (filter 
+                  (fun n => In_dec Address_eqdec n (map fst (snd c))) 
+                  (map fst (snd c')))) certs).
+
+Fixpoint genproof_simple_aux (certs : list Certificate) : list Address :=
+  match certs with
+  | nil => nil
+  | c :: certs' => (genproof_simple_aux_aux c certs') ++ (genproof_simple_aux certs')
+  end.
+
+Definition genproof_simple (certs : list Certificate) : list Address :=
+  nodup Address_eqdec (genproof_simple_aux certs).
+
+Definition genproof := genproof_simple.
+
+Lemma genproof_simple_aux_aux_can_detect v nsigs certs n : 
+  In n (genproof_simple_aux_aux (v, nsigs) certs) <-> 
+  exists v' nsigs',
+    v <> v' /\
+    In (v', nsigs') certs /\
+    In n (map fst nsigs) /\
+    In n (map fst nsigs').
+Proof.
+  induction certs as [ | (v_, nsigs_) certs IH ].
+  - firstorder.
+  - simpl.
+    rewrite -> in_app_iff, -> IH.
+    clear IH.
+    destruct (Value_eqdec v v_) as [ <- | Hvneq ].
+    + firstorder.
+      congruence.
+    + rewrite -> filter_In.
+      (* awkward ... *)
+      assert (in_dec Address_eqdec n (map fst nsigs) <-> In n (map fst nsigs)) as Hp.
+      {
+        unfold is_true.
+        now destruct (in_dec Address_eqdec n (map fst nsigs)).
+      }
+      rewrite -> Hp.
+      intuition firstorder congruence.
+Qed.
+
+Lemma genproof_simple_aux_can_detect certs n : In n (genproof_simple_aux certs) <-> 
+  exists v1 v2 nsigs1 nsigs2,
+    v1 <> v2 /\
+    In (v1, nsigs1) certs /\
+    In (v2, nsigs2) certs /\
+    In n (map fst nsigs1) /\
+    In n (map fst nsigs2).
+Proof.
+  induction certs as [ | (v, nsigs) certs IH ].
+  - firstorder.
+  - simpl.
+    rewrite -> in_app_iff, -> IH, -> genproof_simple_aux_aux_can_detect.
+    clear IH.
+    split.
+    + intros [ (v' & nsigs' & Hvneq & Hin' & Hin_nsigs & Hin_nsigs') | 
+        (v1 & v2 & nsigs1 & nsigs2 & Hvneq & Hin1 & Hin2 & Hin_nsigs1 & Hin_nsigs2) ].
+      * exists v, v', nsigs, nsigs'.
+        intuition.
+      * exists v1, v2, nsigs1, nsigs2.
+        intuition.
+    + intros (v1 & v2 & nsigs1 & nsigs2 & Hvneq & [ Hin1 | Hin1 ] & [ Hin2 | Hin2 ] & Hin_nsigs1 & Hin_nsigs2).
+      all: try congruence.
+      1-2: left.
+      1: exists v2, nsigs2.
+      2: exists v1, nsigs1.
+      1-2: intuition congruence.
+      right.
+      exists v1, v2, nsigs1, nsigs2.
+      intuition.
+Qed.
+
+Lemma genproof_correct : 
+  (forall certs, NoDup (genproof certs)) /\
+  (forall certs n, In n (genproof certs) <-> 
+    exists v1 v2 sig1 sig2 nsigs1 nsigs2,
+      v1 <> v2 /\
+      In (v1, nsigs1) certs /\
+      In (v2, nsigs2) certs /\
+      In (n, sig1) nsigs1 /\
+      In (n, sig2) nsigs2).
+Proof.
+  unfold genproof, genproof_simple.
+  split.
+  - intros. 
+    now apply NoDup_nodup.
+  - intros.
+    rewrite -> nodup_In, -> genproof_simple_aux_can_detect.
+    repeat setoid_rewrite -> in_map_iff.
+    split.
+    + intros (v1 & v2 & nsigs1 & nsigs2 & ? & ? & ? & ((n', sig1) & Htmp1 & ?) & ((n'', sig2) & Htmp2 & ?)).
+      simpl in Htmp1, Htmp2.
+      subst n' n''.
+      now exists v1, v2, sig1, sig2, nsigs1, nsigs2.
+    + intros (v1 & v2 & sig1 & sig2 & nsigs1 & nsigs2 & ? & ? & ? & ? & ?).
+      exists v1, v2, nsigs1, nsigs2.
+      firstorder.
+Qed.
+
+End CertCheckersImpl.
+
+Module Type ACMessage (A : NetAddr) (V : Signable) (P : PKI A V) (TSS : ThresholdSignatureScheme A V)
+  (ACDT : ACDataTypes A V P TSS) <: MessageType.
+
+Import A V P TSS ACDT.
+
+Inductive Message_ := 
+  | SubmitMsg (v : Value) (ls : LightSignature) (s : Signature)
+  | LightConfirmMsg (c : LightCertificate)
+  (* for historical reasons, this remains the name as "ConfirmMsg". *)
+  | ConfirmMsg (c : Certificate).
+
+Definition Message := Message_.
+
+Definition Message_eqdec : forall (m1 m2 : Message), {m1 = m2} + {m1 <> m2}.
+  intros. 
+  decide equality; auto using Signature_eqdec, LightSignature_eqdec, 
+    Value_eqdec, LightCertificate_eqdec, Certificate_eqdec.
+Qed.
+
+End ACMessage.
+
+Module ACMessageImpl (A : NetAddr) (V : Signable) (P : PKI A V) (TSS : ThresholdSignatureScheme A V)
+  (ACDT : ACDataTypes A V P TSS) <: MessageType <: ACMessage A V P TSS ACDT.
+
+Include ACMessage A V P TSS ACDT.
+
+End ACMessageImpl.
